src/Main.fst
@@ -91,9 +91,9 @@ val intro_ind_varraylist_nil (#opened:_)
       (A.varray r `star` R.vptr r1 `star` R.vptr r2 `star` R.vptr r3)
       (fun _ -> ind_varraylist pred1 pred2 pred3 r r1 r2 r3)
       (requires fun h -> A.length r == 0 /\
-        R.sel r1 h == 0sz /\
-        R.sel r2 h == 0sz /\
-        R.sel r3 h == 0sz
+        R.sel r1 h == AL.null_ptr /\
+        R.sel r2 h == AL.null_ptr /\
+        R.sel r3 h == AL.null_ptr
       )
       (ensures fun _ _ _ -> True)
 
@@ -101,15 +101,15 @@ let intro_ind_varraylist_nil pred1 pred2 pred3 r r1 r2 r3 =
   ALG.intro_arraylist_nil
     pred1 pred2 pred3
     r
-    0sz 0sz 0sz;
+    AL.null_ptr AL.null_ptr AL.null_ptr;
 
   let idxs = gget (R.vptr r1 `star` R.vptr r2 `star` R.vptr r3) in
 
-  assert_norm (ind_aux pred1 pred2 pred3 r ((0sz, 0sz), 0sz) ==
-          AL.varraylist pred1 pred2 pred3 r 0 0 0);
+  assert_norm (ind_aux pred1 pred2 pred3 r ((AL.null_ptr, AL.null_ptr), AL.null_ptr) ==
+          AL.varraylist pred1 pred2 pred3 r (US.v AL.null_ptr) (US.v AL.null_ptr) (US.v AL.null_ptr));
   intro_vdep
     (R.vptr r1 `star` R.vptr r2 `star` R.vptr r3)
-    (AL.varraylist pred1 pred2 pred3 r 0 0 0)
+    (AL.varraylist pred1 pred2 pred3 r (US.v AL.null_ptr) (US.v AL.null_ptr) (US.v AL.null_ptr))
     (ind_aux pred1 pred2 pred3 r)
 
 val intro_left_vprop_empty (#opened:_)
@@ -122,9 +122,9 @@ val intro_left_vprop_empty (#opened:_)
       (A.varray (split_l md_region 0sz) `star` R.vptr r1 `star` R.vptr r2 `star` R.vptr r3)
       (fun _ -> SlabsCommon.left_vprop sc slab_region md_bm_region md_region r1 r2 r3 0ul)
       (requires fun h ->
-        R.sel r1 h == 0sz /\
-        R.sel r2 h == 0sz /\
-        R.sel r3 h == 0sz
+        R.sel r1 h == AL.null_ptr /\
+        R.sel r2 h == AL.null_ptr /\
+        R.sel r3 h == AL.null_ptr
       )
       (ensures fun _ _ _ -> True)
 
@@ -234,6 +234,7 @@ let init_struct (sc:sc)
   emp
   (fun scs -> size_class_vprop scs)
   =
+  intro_fits_u32 ();
   let slab_region = mmap_u8 (u32_to_sz (U32.mul metadata_max page_size)) in
   let md_bm_region = mmap_u64 (u32_to_sz (U32.mul metadata_max 4ul)) in
   let md_region = mmap_cell_status (u32_to_sz metadata_max) in
@@ -253,9 +254,9 @@ let init_struct (sc:sc)
   let ptr_empty = mmap_ptr_us () in
   let ptr_full = mmap_ptr_us () in
 
-  R.write ptr_partial 0sz;
-  R.write ptr_empty 0sz;
-  R.write ptr_full 0sz;
+  R.write ptr_partial AL.null_ptr;
+  R.write ptr_empty AL.null_ptr;
+  R.write ptr_full AL.null_ptr;
 
   intro_left_vprop_empty sc (A.split_r slab_region 0sz) md_bm_region md_region ptr_empty ptr_partial ptr_full;
 
