src/SlabsCommon.fst
@@ -365,6 +365,7 @@ let pack_3
       (left_vprop size_class slab_region md_bm_region md_region r1 r2 r3)
   )
   (requires fun h0 ->
+    U32.v md_count_v <> AL.null /\
     sel md_count h0 == md_count_v /\
     ALG.dataify (AL.v_arraylist pred1 pred2 pred3 (A.split_l md_region (u32_to_sz md_count_v)) (US.v idx1) (US.v idx2) (US.v idx3) h0) `Seq.equal` Ghost.reveal md_region_lv /\
     sel r1 h0 == idx1 /\
